(WIP) Proving twin execution

TwinProperty.v
@@ -11,49 +11,61 @@ Require Import Behaviors.
 Require Import Memory.
 Require Import State.
 Require Import SmallStep.
+Require Import Reordering.
 
 
 Module Ir.
 
-Definition twin_state (st1 st2:Ir.Config.t) (blkid:Ir.blockid) :=
+(* Definition of 'twin' states.*)
+Definition twin_state (st1 st2:Ir.Config.t) (blkid:Ir.blockid):Prop :=
   Ir.Config.eq_wom st1 st2 /\
-  exists mb1 mb2,
-    Some mb1 = Ir.Memory.get (Ir.Config.m st1) blkid /\
-    Some mb2 = Ir.Memory.get (Ir.Config.m st2) blkid /\
-    (Ir.MemBlock.bt mb1) = (Ir.MemBlock.bt mb2) /\
-    (Ir.MemBlock.r mb1) = (Ir.MemBlock.r mb2) /\
-    (Ir.MemBlock.n mb1) = (Ir.MemBlock.n mb2) /\
-    (Ir.MemBlock.a mb1) = (Ir.MemBlock.a mb2) /\
-    (Ir.MemBlock.c mb1) = (Ir.MemBlock.c mb2) /\
-    Permutation (Ir.MemBlock.P mb1) (Ir.MemBlock.P mb2) /\
-    Ir.MemBlock.P mb1 <> Ir.MemBlock.P mb2.
+  Ir.Memory.mt (Ir.Config.m st1) = Ir.Memory.mt (Ir.Config.m st2) /\
+  Ir.Memory.calltimes (Ir.Config.m st1) = Ir.Memory.calltimes (Ir.Config.m st2) /\
+  Ir.Memory.fresh_bid (Ir.Config.m st1) = Ir.Memory.fresh_bid (Ir.Config.m st2) /\
+  forall bid',
+    (forall (HMATCH:bid' = blkid),
+        exists mb1 mb2,
+          Some mb1 = Ir.Memory.get (Ir.Config.m st1) blkid /\
+          Some mb2 = Ir.Memory.get (Ir.Config.m st2) blkid /\
+          (Ir.MemBlock.bt mb1) = (Ir.MemBlock.bt mb2) /\
+          (Ir.MemBlock.r mb1) = (Ir.MemBlock.r mb2) /\
+          (Ir.MemBlock.n mb1) = (Ir.MemBlock.n mb2) /\
+          (Ir.MemBlock.a mb1) = (Ir.MemBlock.a mb2) /\
+          (Ir.MemBlock.c mb1) = (Ir.MemBlock.c mb2) /\
+          Permutation (Ir.MemBlock.P mb1) (Ir.MemBlock.P mb2) /\
+          List.hd 0 (Ir.MemBlock.P mb1) <> List.hd 0 (Ir.MemBlock.P mb2))
+    /\
+    (forall (HMATCH:bid' <> blkid),
+        Ir.Memory.get (Ir.Config.m st1) bid' =
+        Ir.Memory.get (Ir.Config.m st2) bid').
 
-(* Definition of a 'twin' step. *)
-Inductive twin_step:
+(* Given two small step results (e.g. success/goes wrong/oom/program end),
+   they are twin if it satisfies one of the followings. *)
+Inductive twin_sresult:
 Ir.SmallStep.step_res -> Ir.SmallStep.step_res -> Ir.blockid -> Prop :=
   | ts_success:
       forall st1 st2 (sr1 sr2:Ir.SmallStep.step_res) (e1 e2:Ir.event) blkid
              (HSR1:sr1 = Ir.SmallStep.sr_success e1 st1)
              (HSR2:sr2 = Ir.SmallStep.sr_success e2 st2)
              (HTWIN:twin_state st1 st2 blkid),
-        twin_step sr1 sr2 blkid
+        twin_sresult sr1 sr2 blkid
   | ts_goes_wrong:
       forall sr1 sr2 blkid
              (HSR1:sr1 = Ir.SmallStep.sr_goes_wrong)
              (HSR1:sr2 = Ir.SmallStep.sr_goes_wrong),
-        twin_step sr1 sr2 blkid
+        twin_sresult sr1 sr2 blkid
   | ts_oom:
       forall sr1 sr2 blkid
              (HSR1:sr1 = Ir.SmallStep.sr_oom)
              (HSR1:sr2 = Ir.SmallStep.sr_oom),
-        twin_step sr1 sr2 blkid
+        twin_sresult sr1 sr2 blkid
   | ts_prog_finish:
       forall sr1 sr2 blkid v
              (HSR1:sr1 = Ir.SmallStep.sr_prog_finish v)
              (HSR1:sr2 = Ir.SmallStep.sr_prog_finish v),
-        twin_step sr1 sr2 blkid.
+        twin_sresult sr1 sr2 blkid.
 
-
+(* A memory block blkid is observed at state st if.. *)
 Inductive observes_block (md:Ir.IRModule.t) (st:Ir.Config.t) (blkid:Ir.blockid):Prop :=
   | ob_by_ptrtoint:
       forall r op1 retty o
@@ -99,16 +111,823 @@ Inductive observes_block (md:Ir.IRModule.t) (st:Ir.Config.t) (blkid:Ir.blockid):
              (HOP2:Some (Ir.ptr (Ir.pphy o2 I2 cid2)) = Ir.Config.get_val st op1), 
         observes_block md st blkid.
 
+(* A value is possibly a guessed pointer if it is a physical pointer. *)
+Inductive possibly_guessedptr (v:Ir.val):Prop :=
+| pg_phy: forall o I cid (HPHY: v = Ir.ptr (Ir.pphy o I cid)),
+    possibly_guessedptr v.
+
+(* Memory access from a possibly guessed pointer if.. *)
+Inductive memaccess_from_possibly_guessedptr (md:Ir.IRModule.t) (st:Ir.Config.t)
+:Prop :=
+  | gp_store:
+      forall valty opval opptr vptr
+        (HOPPTR: Some vptr = Ir.Config.get_val st opptr)
+        (HGUESSED: possibly_guessedptr vptr)
+        (HINST: Some (Ir.Inst.istore valty opval opptr) =
+                Ir.Config.cur_inst md st),
+        memaccess_from_possibly_guessedptr md st
+  | gp_load:
+      forall retty opval opptr vptr
+        (HOPPTR: Some vptr = Ir.Config.get_val st opptr)
+        (HGUESSED: possibly_guessedptr vptr)
+        (HINST: Some (Ir.Inst.iload retty opval opptr) =
+                Ir.Config.cur_inst md st),
+        memaccess_from_possibly_guessedptr md st
+  | gp_free:
+      forall opptr vptr
+        (HOPPTR: Some vptr = Ir.Config.get_val st opptr)
+        (HGUESSED: possibly_guessedptr vptr)
+        (HINST: Some (Ir.Inst.ifree opptr) =
+                Ir.Config.cur_inst md st),
+        memaccess_from_possibly_guessedptr md st.
+
+Lemma eq_wom_refl:
+  forall st1,
+    Ir.Config.eq_wom st1 st1.
+Proof.
+  intros.
+  split.
+  { apply Ir.Stack.eq_refl.  }
+  { split; congruence. }
+Qed.
+
+Lemma eq_wom_sym:
+  forall st1 st2 (HEQ:Ir.Config.eq_wom st1 st2),
+    Ir.Config.eq_wom st2 st1.
+Proof.
+  intros.
+  inv HEQ.
+  inv H0.
+  split.
+  { apply Ir.Stack.eq_symm. eassumption. }
+  { split; congruence. }
+Qed.
+
+Lemma eq_wom_update_m:
+  forall st1 st2 (HEQ:Ir.Config.eq_wom st1 st2) m1 m2,
+    Ir.Config.eq_wom (Ir.Config.update_m st1 m1) (Ir.Config.update_m st2 m2).
+Proof.
+  intros.
+  unfold Ir.Config.update_m.
+  inv HEQ.
+  inv H0.
+  unfold Ir.Config.eq_wom.
+  simpl.
+  split. assumption.
+  split; assumption.
+Qed.
+
+Lemma twin_state_sym:
+  forall st1 st2 blkid (HTWIN:twin_state st1 st2 blkid),
+    twin_state st2 st1 blkid.
+Proof.
+  intros.
+  inv HTWIN.
+  split.
+  { apply eq_wom_sym. assumption. }
+  inv H0.
+  split. congruence.
+  inv H2.
+  split. congruence.
+  inv H3.
+  split. congruence.
+  intros.
+  assert (H4' := H4 bid'). inv H4'. clear H4.
+  split.
+  { intros HH. subst bid'.
+    assert (HH2 := eq_refl blkid).
+    apply H3 in HH2.
+    destruct HH2 as [mb1 HH2].
+    destruct HH2 as [mb2 HH2].
+    inv HH2.
+    destruct H6.
+    destruct H7.
+    destruct H8.
+    destruct H9.
+    destruct H10.
+    destruct H11.
+    destruct H12.
+    exists mb2, mb1.
+    repeat (split; try congruence).
+    apply Permutation_sym. congruence.
+  }
+  { intros. apply H5 in HMATCH.
+    congruence.
+  }
+Qed.
+
+Lemma twin_state_get_funid_eq:
+  forall (st1 st2:Ir.Config.t) c blkid
+         (HTWIN:twin_state st1 st2 blkid),
+    Ir.Config.get_funid st1 c = Ir.Config.get_funid st2 c.
+Proof.
+  intros.
+  unfold Ir.Config.get_funid.
+  inv HTWIN.
+  inv H.
+  inv H2.
+  rewrite H.
+  reflexivity.
+Qed.
+
+Lemma twin_state_cur_fdef_pc_eq:
+  forall (md:Ir.IRModule.t) (st1 st2:Ir.Config.t) blkid
+         (HTWIN:twin_state st1 st2 blkid),
+    Ir.Config.cur_fdef_pc md st1 = Ir.Config.cur_fdef_pc md st2.
+Proof.
+  intros.
+  dup HTWIN.
+  unfold Ir.Config.cur_fdef_pc.
+  inv HTWIN.
+  inv H0.
+  inv H1.
+  inv H.
+  des_ifs; try (inv H0; fail).
+  try ( unfold Ir.Stack.eq in H0; inv H0;
+    simpl in H6; inv H6; inv H0;
+    rewrite twin_state_get_funid_eq with (st2 := st2) (blkid := blkid) in Heq0;
+      try assumption;
+    rewrite Heq3 in Heq0; inv Heq0;
+    rewrite Heq4 in Heq1; inv Heq1;
+    reflexivity
+  ).
+  { unfold Ir.Stack.eq in H0.
+    inv H0.
+    simpl in H6.
+    inv H6. inv H0.
+    rewrite twin_state_get_funid_eq with (st2 := st2) (blkid := blkid) in Heq0;
+      try assumption.
+    rewrite Heq3 in Heq0. inv Heq0.
+    rewrite Heq4 in Heq1. inv Heq1.
+  }
+  { unfold Ir.Stack.eq in H0.
+    inv H0.
+    simpl in H6.
+    inv H6. inv H0.
+    rewrite twin_state_get_funid_eq with (st2 := st2) (blkid := blkid) in Heq0;
+      try assumption.
+    rewrite Heq3 in Heq0. inv Heq0.
+  }
+  { unfold Ir.Stack.eq in H0.
+    inv H0.
+    simpl in H6.
+    inv H6. inv H0.
+    rewrite twin_state_get_funid_eq with (st2 := st2) (blkid := blkid) in Heq0;
+      try assumption.
+    rewrite Heq3 in Heq0. inv Heq0.
+    rewrite Heq4 in Heq1. inv Heq1.
+  }
+  { unfold Ir.Stack.eq in H0.
+    inv H0.
+    simpl in H6.
+    inv H6. inv H0.
+    rewrite twin_state_get_funid_eq with (st2 := st2) (blkid := blkid) in Heq0;
+      try assumption.
+    rewrite Heq2 in Heq0. inv Heq0.
+  }
+Qed.
+
+Lemma twin_state_cur_inst_eq:
+  forall (md:Ir.IRModule.t) (st1 st2:Ir.Config.t) blkid
+         (HTWIN:twin_state st1 st2 blkid),
+    Ir.Config.cur_inst md st1 = Ir.Config.cur_inst md st2.
+Proof.
+  intros.
+  inv HTWIN.
+  unfold Ir.Config.cur_inst.
+  inv H.
+  unfold Ir.Config.cur_fdef_pc.
+  unfold Ir.Stack.eq in H1.
+  destruct (Ir.Config.s st1);
+    destruct (Ir.Config.s st2).
+  { reflexivity. }
+  { inv H1. }
+  { inv H1. }
+  { inv H1. inv H5. inv H1.
+    destruct p. destruct p0. simpl in H. subst c.
+    simpl in H3.
+    destruct p. destruct p0.
+    simpl in H3. subst p.
+    simpl in H4.
+    unfold Ir.Config.get_funid.
+    inv H2.
+    rewrite H.
+    des_ifs.
+  }
+Qed.
+
+Lemma twin_state_get_val_eq:
+  forall (st1 st2:Ir.Config.t) blkid r
+         (HTWIN:twin_state st1 st2 blkid),
+    Ir.Config.get_val st1 r = Ir.Config.get_val st2 r.
+Proof.
+  intros.
+  inv HTWIN.
+  unfold Ir.Config.get_val.
+  destruct r; try reflexivity.
+  unfold Ir.Config.get_rval.
+  inv H.
+  unfold Ir.Stack.eq in H1.
+  destruct (Ir.Config.s st1);
+    destruct (Ir.Config.s st2).
+  { reflexivity. }
+  { inv H1. }
+  { inv H1. }
+  { inv H1. inv H5. inv H1.
+    destruct p. destruct p0. simpl in H. subst c.
+    simpl in H3.
+    destruct p. destruct p0.
+    simpl in H3. subst p.
+    simpl in H4.
+    unfold Ir.Regfile.eq in H4.
+    apply H4.
+  }
+Qed.
+
+Lemma twin_state_update_rval: 
+  forall (st1 st2:Ir.Config.t) blkid r v
+         (HTWIN:twin_state st1 st2 blkid),
+    twin_state (Ir.Config.update_rval st1 r v)
+               (Ir.Config.update_rval st2 r v) blkid.
+Proof.
+  intros.
+  inv HTWIN.
+  inv H.
+  unfold Ir.Config.update_rval.
+  des_ifs; try (inv H1; fail).
+  { split.
+    { split. rewrite Heq, Heq0. assumption.
+      assumption. }
+    { apply H0. }
+  }
+  { inv H1.
+    simpl in H5. inv H5. inv H1.
+    destruct H0.
+    destruct H0.
+    destruct H1.
+    split.
+    { split.
+      { simpl. unfold Ir.Stack.eq. simpl.
+        apply List.Forall2_cons. simpl.
+        split. congruence. split . congruence.
+        apply Ir.Regfile.update_eq. assumption.
+        assumption.
+      }
+      { assumption. }
+    }
+    simpl.
+    split. congruence.
+    split. congruence.
+    split. congruence.
+    intros.
+    assert (H4' := H4 bid'). clear H4.
+    split.
+    { intros HH. simpl. subst bid'.
+      destruct H4'. assert (HDUMMY: blkid = blkid) by reflexivity.
+      apply H4 in HDUMMY. clear H4.
+      destruct HDUMMY as [mb1 HDUMMY].
+      destruct HDUMMY as [mb2 HDUMMY].
+      exists mb1. exists mb2.
+      assumption.
+    }
+    { intros HH. destruct H4'.
+      apply H5 in HH. assumption.
+    }
+  }
+Qed.
+
+Lemma twin_state_update_pc:
+  forall (st1 st2:Ir.Config.t) blkid pc0
+         (HTWIN:twin_state st1 st2 blkid),
+    twin_state (Ir.Config.update_pc st1 pc0)
+               (Ir.Config.update_pc st2 pc0) blkid.
+Proof.
+  intros.
+  inv HTWIN.
+  inv H.
+  unfold Ir.Config.update_pc.
+  des_ifs; try (inv H1; fail).
+  { split.
+    { split. rewrite Heq, Heq0. assumption.
+      assumption. }
+    { apply H0. }
+  }
+  { inv H1.
+    simpl in H5. inv H5. inv H1.
+    split.
+    { split.
+      { simpl. unfold Ir.Stack.eq. simpl.
+        apply List.Forall2_cons. simpl.
+        split. congruence. split . congruence.
+        assumption.
+        assumption.
+      }
+      { assumption. }
+    }
+    simpl in *.
+    destruct H0.
+    destruct H0.
+    destruct H1.
+    split. congruence.
+    split. congruence.
+    split. congruence.
+    intros.
+    assert (H4' := H4 bid').
+    clear H4. destruct H4'.
+    split.
+    { intros. eauto. }
+    { intros. eauto. }
+  }
+Qed.
+
+Lemma twin_state_incrpc:
+  forall md (st1 st2:Ir.Config.t) blkid
+         (HTWIN:twin_state st1 st2 blkid),
+    twin_state (Ir.SmallStep.incrpc md st1)
+               (Ir.SmallStep.incrpc md st2) blkid.
+Proof.
+  intros.
+  dup HTWIN.
+  inv HTWIN.
+  inv H.
+  unfold Ir.SmallStep.incrpc.
+  rewrite twin_state_cur_fdef_pc_eq with (st2 := st2) (blkid := blkid);
+    try assumption.
+  des_ifs; try (inv H1; fail).
+  apply twin_state_update_pc.
+  assumption.
+Qed.
+
+Lemma twin_state_update_reg_and_incrpc:
+  forall md (st1 st2:Ir.Config.t) blkid r v
+         (HTWIN:twin_state st1 st2 blkid),
+    twin_state (Ir.SmallStep.update_reg_and_incrpc md st1 r v)
+               (Ir.SmallStep.update_reg_and_incrpc md st2 r v) blkid.
+Proof.
+  intros.
+  unfold Ir.SmallStep.update_reg_and_incrpc.
+  apply twin_state_incrpc.
+  apply twin_state_update_rval.
+  assumption.
+Qed.
+
+Lemma twin_state_p2N_eq:
+  forall st1 st2 b blkid n o
+         (HTWIN: twin_state st1 st2 blkid)
+         (HNEQ:b <> blkid),
+    Ir.SmallStep.p2N (Ir.plog b o) (Ir.Config.m st1) n =
+    Ir.SmallStep.p2N (Ir.plog b o) (Ir.Config.m st2) n.
+Proof.
+  intros.
+  inv HTWIN.
+  destruct H0.
+  destruct H1.
+  destruct H2.
+  assert (HH := H3 b).
+  clear H3.
+  destruct HH. clear H3.
+  apply H4 in HNEQ. clear H4.
+  unfold Ir.SmallStep.p2N.
+  unfold LoadStore.Ir.log_to_phy.
+  rewrite HNEQ.
+  reflexivity.
+Qed.
+
+Lemma twin_state_gep_eq:
+  forall st1 st2 b blkid n t o inb
+         (HTWIN: twin_state st1 st2 blkid),
+    Ir.SmallStep.gep (Ir.plog b o) n t (Ir.Config.m st1) inb =
+    Ir.SmallStep.gep (Ir.plog b o) n t (Ir.Config.m st2) inb.
+Proof.
+  intros.
+  destruct HTWIN.
+  destruct H0.
+  destruct H1.
+  destruct H2.
+  assert (HH := H3 b).
+  clear H3.
+  destruct HH.
+  destruct (b =? blkid) eqn:HBLKID.
+  { rewrite PeanoNat.Nat.eqb_eq in HBLKID.
+    dup HBLKID.
+    apply H3 in HBLKID.
+    subst b.
+    clear H3. destruct HBLKID. destruct H3.
+    destruct H3.
+    destruct H5.
+    unfold Ir.SmallStep.gep.
+    destruct inb.
+    { rewrite <- H3. rewrite <- H5.
+      assert (HINB: forall o', Ir.MemBlock.inbounds o' x = Ir.MemBlock.inbounds o' x0).
+      { intros.
+        unfold Ir.MemBlock.inbounds.
+        destruct H6.
+        destruct H7.
+        destruct H8.
+        rewrite H8. reflexivity. }
+      rewrite HINB.
+      rewrite HINB.
+      reflexivity.
+    }
+    { reflexivity. }
+  }
+  { unfold Ir.SmallStep.gep.
+    rewrite PeanoNat.Nat.eqb_neq in HBLKID.
+    apply H4 in HBLKID.
+    rewrite HBLKID.
+    reflexivity.
+  }
+Qed.
+
+
+(*******************************************************
+                 Main Theorems 
+ *******************************************************)
+
+Lemma regfile_get_update:
+  forall rf r v,
+    Ir.Regfile.get (Ir.Regfile.update rf r v) r = Some v.
+Proof.
+  intros.
+  unfold Ir.Regfile.get.
+  unfold Ir.Regfile.update.
+  unfold list_find_key.
+  simpl.
+  rewrite PeanoNat.Nat.eqb_refl. reflexivity.
+Qed.
+
+Lemma get_val_update_reg_and_incrpc_samereg:
+  forall md st r v
+         (HSTACK:Ir.Config.s st <> nil), (* stack is not empty. *)
+    Ir.Config.get_val (Ir.SmallStep.update_reg_and_incrpc md st r v)
+                      (Ir.opreg r) =
+    Some v.
+Proof.
+  intros.
+  unfold Ir.SmallStep.update_reg_and_incrpc.
+  unfold Ir.Config.get_val.
+  unfold Ir.Config.get_rval.
+  unfold Ir.SmallStep.incrpc.
+  unfold Ir.Config.cur_fdef_pc.
+  unfold Ir.Config.get_funid.
+  unfold Ir.Config.update_rval.
+  destruct (Ir.Config.s st); try congruence.
+  destruct p. destruct p.
+  simpl.
+  destruct (list_find_key (Ir.Config.cid_to_f st) c).
+  { simpl. apply regfile_get_update. }
+  { simpl.
+    des_ifs.
+    - simpl in Heq. inv Heq. apply regfile_get_update.
+    - simpl in Heq. inv Heq. apply regfile_get_update.
+    - simpl in Heq. inv Heq. apply regfile_get_update.
+  }
+Qed.  
+
+Lemma disjoint_range_sym:
+  forall r1 r2, disjoint_range r1 r2 = disjoint_range r2 r1.
+Proof.
+  intros. unfold disjoint_range.
+  destruct r1. destruct r2.
+  intuition.
+Qed.
+
+(* If malloc succeeds, it always creates twin-state. *)
+Theorem malloc_creates_twin_state:
+  forall (md:Ir.IRModule.t) (st st'1: Ir.Config.t) r retty opsz e'1
+         (HCUR: Some (Ir.Inst.imalloc r retty opsz) = Ir.Config.cur_inst md st)
+         (HNEXT: Ir.SmallStep.inst_step md st (Ir.SmallStep.sr_success e'1 st'1)),
+    (* malloc can return NULL, or *)
+    Some (Ir.ptr (Ir.NULL)) = Ir.Config.get_val st'1 (Ir.opreg r) \/
+    (* malloc reutrn (bid, 0), and malloc can nondeterministically make
+       twin state with respect to bid as well *)
+    exists st'2 bid,
+      Some (Ir.ptr (Ir.plog bid 0)) = Ir.Config.get_val st'1 (Ir.opreg r) /\
+      Ir.SmallStep.inst_step md st (Ir.SmallStep.sr_success e'1 st'2) /\
+      twin_state st'1 st'2 bid.
+Proof.
+  intros.
+  assert (HSTACK:Ir.Config.s st <> []).
+  { unfold Ir.Config.cur_inst in HCUR.
+    unfold Ir.Config.cur_fdef_pc in HCUR.
+    des_ifs. }
+  inv HNEXT.
+  { unfold Ir.SmallStep.inst_det_step in HNEXT0.
+    des_ifs. }
+  { (* returned NULL*)
+    left.
+    rewrite <- HCUR in HCUR0. inv HCUR0.
+    rewrite get_val_update_reg_and_incrpc_samereg. reflexivity. assumption. }
+  { (* malloc succeeded. *)
+    right.
+    rewrite <- HCUR in HCUR0.
+    inv HCUR0.
+    (* Let's make P' which is permutated P. *)
+    dup HMBWF.
+    assert (HMBWF' := HMBWF (Ir.Memory.mt (Ir.Config.m st))).
+    clear HMBWF.
+    inv HMBWF'.
+    rewrite get_val_update_reg_and_incrpc_samereg.
+    simpl in *.
+    destruct P as [ | p1 P]; try (inv wf_twin; fail).
+    destruct P as [ | p2 P]; try (inv wf_twin; fail).
+    exists (Ir.SmallStep.update_reg_and_incrpc md
+        (Ir.Config.update_m st
+          (fst (Ir.Memory.new (Ir.Config.m st) (Ir.heap) (N.to_nat nsz)
+                       (Ir.SYSALIGN) (List.repeat Ir.Byte.poison (N.to_nat nsz))
+                       (p2::p1::P))))
+        r (Ir.ptr (Ir.plog l 0))).
+    exists l.
+    split.
+    { reflexivity. }
+    split.
+    { eapply Ir.SmallStep.s_malloc with (P := p2::p1::P).
+      eassumption. reflexivity. eassumption. eassumption. reflexivity.
+      { clear wf_tcond.
+        clear wf_poslen wf_align wf_inmem wf_notnull wf_disj wf_twin.
+        intros.
+        assert (HMBWF0' := HMBWF0 begt).
+        inv HMBWF0'.
+        simpl in *.
+        split.
+        { intros. simpl in *. congruence. }
+        { simpl. assumption. }
+        { simpl. assumption. }
+        { simpl. intros.
+          apply wf_align. intuition. }
+        { simpl. intros. apply wf_inmem. intuition. }
+        { simpl. intros. apply wf_notnull. intuition. }
+        { simpl. repeat (rewrite andb_true_iff).
+          repeat (rewrite andb_true_iff in wf_disj).
+          inv wf_disj. inv H. inv H0.
+          split.
+          split.
+          { rewrite disjoint_range_sym. assumption. }
+          { assumption. }
+          split.
+          { assumption. }
+          { assumption. }
+        }
+        { simpl. assumption. }
+      }
+      { unfold Ir.Memory.allocatable in *.
+        simpl in HDISJ.
+        simpl.
+        { simpl. repeat (rewrite andb_true_iff).
+          repeat (rewrite andb_true_iff in HDISJ).
+          inv HDISJ. inv H. inv H0.
+          split.
+          split.
+          { rewrite disjoint_range_sym. assumption. }
+          { assumption. }
+          split.
+          { assumption. }
+          { assumption. }
+        }
+      }
+      { unfold Ir.Memory.new.
+        simpl.
+        unfold Ir.Memory.new in HNEW.
+        inv HNEW.
+        reflexivity.
+      }
+    }
+    { unfold Ir.Memory.new in HNEW.
+      inv HNEW.
+      simpl.
+      unfold twin_state.
+      split.
+      { 
+        rewrite Ir.Reordering.update_reg_and_incrpc_update_m.
+        rewrite Ir.Reordering.update_reg_and_incrpc_update_m.
+        apply eq_wom_update_m.
+        apply eq_wom_refl.
+      }
+      { repeat (rewrite Ir.Reordering.update_reg_and_incrpc_update_m).
+        repeat (rewrite Ir.Reordering.m_update_m).
+        simpl.
+        split. reflexivity.
+        split. reflexivity.
+        split. reflexivity.
+        split.
+        { intros H0.
+          subst bid'.
+          eexists. eexists.
+          split.
+          { unfold Ir.Memory.get.
+            simpl. rewrite PeanoNat.Nat.eqb_refl. reflexivity. }
+          split.
+          { unfold Ir.Memory.get. simpl.
+            rewrite PeanoNat.Nat.eqb_refl. reflexivity. }
+          simpl.
+          split. reflexivity.
+          split. reflexivity.
+          split. reflexivity.
+          split. reflexivity.
+          split. reflexivity.
+          split. apply perm_swap.
+          { (* p1 <> p2 comes from wf_disj. *)
+            simpl in wf_disj.
+            rewrite andb_true_iff in wf_disj.
+            rewrite andb_true_iff in wf_disj.
+            rewrite andb_true_iff in wf_disj.
+            inv wf_disj. inv H.
+            unfold disjoint_range in H1.
+            rewrite orb_true_iff in H1.
+            rewrite Nat.leb_le in H1.
+            rewrite Nat.leb_le in H1.
+            destruct (N.to_nat nsz). omega.
+            rewrite Nat.add_succ_r in H1.
+            rewrite Nat.add_succ_r in H1.
+            rewrite Nat.le_succ_l in H1.
+            rewrite Nat.le_succ_l in H1.
+            omega.
+          }
+        }
+        { intros.
+          unfold Ir.Memory.get.
+          simpl. apply not_eq_sym in HMATCH.
+          rewrite <- PeanoNat.Nat.eqb_neq in HMATCH.
+          rewrite HMATCH.
+          reflexivity.
+        }
+      }
+    }
+    unfold Ir.Config.update_m.
+    simpl. assumption.
+  }
+  { rewrite <- HCUR in HCUR0. congruence. }
+  { rewrite <- HCUR in HCUR0. congruence. }
+Qed.
+      
+
+Ltac thats_it := apply twin_state_update_reg_and_incrpc;
+            assumption.
+
+Lemma twin_execution_unidir:
+  forall (md:Ir.IRModule.t) (blkid:Ir.blockid)
+    (* If block blkid is never observed.. *)
+    (HNEVER_OBSERVED: forall (st:Ir.Config.t), ~ observes_block md st blkid),
+
+    forall (st1 st2:Ir.Config.t) (sr1 sr2:Ir.SmallStep.step_res)
+           (* Input state st1 and st2 are twin-state. *)
+           (HTWIN:twin_state st1 st2 blkid)
+           (* Current instruction wouldn't do memory access
+              from a guessed pointer. *)
+           (HNOGUESSEDACCESS:~ memaccess_from_possibly_guessedptr md st1),
+    (* one way dir *)  
+    forall sr1 (HSTEP1:Ir.SmallStep.inst_step md st1 sr1),
+          exists sr2, Ir.SmallStep.inst_step md st2 sr2 /\
+                      twin_sresult sr1 sr2 blkid.
+Proof.
+  intros.
+  inv HSTEP1.
+  { unfold Ir.SmallStep.inst_det_step in HNEXT.
+    remember (Ir.Config.cur_inst md st1) as oi1.
+    destruct oi1 as [i1 | ].
+    { erewrite twin_state_cur_inst_eq in Heqoi1; try (apply HTWIN; fail).
+      destruct i1; inv HNEXT; eexists.
+      { (* binop *)
+        split.
+        { apply Ir.SmallStep.s_det. unfold Ir.SmallStep.inst_det_step.
+          rewrite <- Heqoi1.
+          reflexivity. }
+        { erewrite twin_state_get_val_eq with (st1 := st1);
+            try (apply HTWIN; fail).
+          erewrite twin_state_get_val_eq with (st1 := st1);
+            try (apply HTWIN; fail).
+          eapply ts_success.
+          { reflexivity. }
+          { reflexivity. }
+          { thats_it. }
+        }
+      }
+      { (* psub *)
+        split.
+        { apply Ir.SmallStep.s_det. unfold Ir.SmallStep.inst_det_step.
+          rewrite <- Heqoi1.
+          reflexivity. }
+        { erewrite twin_state_get_val_eq with (st1 := st1);
+            try (apply HTWIN; fail).
+          erewrite twin_state_get_val_eq with (st1 := st1);
+            try (apply HTWIN; fail).
+          eapply ts_success.
+          { reflexivity. }
+          { reflexivity. }
+          { destruct t; try thats_it.
+            destruct (Ir.Config.get_val st2 o) eqn:Hop1; try thats_it.
+            destruct v; try thats_it.
+            destruct (Ir.Config.get_val st2 o0) eqn:Hop2; try thats_it.
+            destruct v; try thats_it.
+            destruct p; destruct p0.
+            { unfold Ir.SmallStep.psub. thats_it. }
+            { destruct (b =? blkid) eqn:HBLKID.
+              { (* observed. *)
+                rewrite PeanoNat.Nat.eqb_eq in HBLKID.
+                subst b.
+                assert (HNO2 := HNEVER_OBSERVED st2).
+                assert (Heqoi2 := Heqoi1).
+                rewrite twin_state_cur_inst_eq with (st2 := st1) (blkid := blkid)
+                  in Heqoi2 by (apply twin_state_sym in HTWIN; assumption).
+                assert (observes_block md st2 blkid).
+                { eapply ob_by_psub_l.
+                  { rewrite Heqoi1. reflexivity. }
+                  { rewrite Hop1. reflexivity. }
+                  { rewrite Hop2. reflexivity. }
+                }
+                congruence.
+              }
+              { unfold Ir.SmallStep.psub.
+                rewrite PeanoNat.Nat.eqb_neq in HBLKID.
+                rewrite twin_state_p2N_eq with (st2 := st2) (blkid := blkid);
+                  try assumption.
+                thats_it.
+              }
+            }
+            { destruct (b =? blkid) eqn:HBLKID.
+              { (* observed. *)
+                rewrite PeanoNat.Nat.eqb_eq in HBLKID.
+                subst b.
+                assert (HNO2 := HNEVER_OBSERVED st2).
+                assert (Heqoi2 := Heqoi1).
+                rewrite twin_state_cur_inst_eq with (st2 := st1) (blkid := blkid)
+                  in Heqoi2 by (apply twin_state_sym in HTWIN; assumption).
+                assert (observes_block md st2 blkid).
+                { eapply ob_by_psub_r.
+                  { rewrite Heqoi1. reflexivity. }
+                  { rewrite Hop2. reflexivity. }
+                  { rewrite Hop1. reflexivity. }
+                }
+                congruence.
+              }
+              { unfold Ir.SmallStep.psub.
+                rewrite PeanoNat.Nat.eqb_neq in HBLKID.
+                rewrite twin_state_p2N_eq with (st2 := st2) (blkid := blkid);
+                  try assumption.
+                thats_it.
+              }
+            }
+            { unfold Ir.SmallStep.psub. thats_it. }
+        }
+      }
+    }
+    { (* gep *)
+      split.
+      { apply Ir.SmallStep.s_det. unfold Ir.SmallStep.inst_det_step.
+        rewrite <- Heqoi1.
+        reflexivity. }
+      { erewrite twin_state_get_val_eq with (st1 := st1);
+          try (apply HTWIN; fail).
+        erewrite twin_state_get_val_eq with (st1 := st1);
+          try (apply HTWIN; fail).
+        eapply ts_success.
+        { reflexivity. }
+        { reflexivity. }
+        { destruct t; try thats_it.
+          destruct (Ir.Config.get_val st2 o) eqn:Hop1; try thats_it.
+          destruct v; try thats_it.
+          destruct (Ir.Config.get_val st2 o0) eqn:Hop2; try thats_it.
+          destruct v; try thats_it.
+          destruct p.
+          { erewrite twin_state_gep_eq; try eassumption.
+            thats_it.
+          }
+          { unfold Ir.SmallStep.gep. thats_it. }
+        }
+      }
+    }
+    { (* load *)
+      split.
+      { apply Ir.SmallStep.s_det. unfold Ir.SmallStep.inst_det_step.
+        rewrite <- Heqoi1.
+        reflexivity. }
+      { erewrite twin_state_get_val_eq with (st1 := st1);
+          try (apply HTWIN; fail).
+        erewrite twin_state_get_val_eq with (st1 := st1);
+          try (apply HTWIN; fail).
+        eapply ts_success.
+      
+Qed.
 
 Theorem twin_property:
   forall (md:Ir.IRModule.t) (blkid:Ir.blockid)
+    (* If block blkid is never observed.. *)
     (HNEVER_OBSERVED: forall (st:Ir.Config.t), ~ observes_block md st blkid),
+
     forall (st1 st2:Ir.Config.t) (sr1 sr2:Ir.SmallStep.step_res)
-           (HTWIN:twin_state st1 st2 blkid)
-           (HSTEP1:Ir.SmallStep.inst_step md st1 sr1)
-           (HSTEP2:Ir.SmallStep.inst_step md st2 sr2),
-      twin_step sr1 sr2 blkid.
+           (* Input state st1 and st2 are twin-state. *)
+           (HTWIN:twin_state st1 st2 blkid),
+      (* Bisimulation. *)
+      (forall sr1 (HSTEP1:Ir.SmallStep.inst_step md st1 sr1),
+          exists sr2, Ir.SmallStep.inst_step md st2 sr2 /\
+                      twin_sresult sr1 sr2 blkid) /\
+      (forall sr2 (HSTEP1:Ir.SmallStep.inst_step md st2 sr2),
+          exists sr1, Ir.SmallStep.inst_step md st1 sr1 /\
+                      twin_sresult sr1 sr2 blkid).
 Proof.
+  intros.
+
+  
 Qed.
 
 Definition
